Hoare/Multistep_Hoare.thy
@@ -1,4 +1,5 @@
 theory Multistep_Hoare imports Hoare "../Semantics/Gensyn_Sem_Small"
+"../Gensyn_Descend_Facts"
 begin
 
 (* Idea here:
@@ -198,182 +199,456 @@ proof(rule GVTI)
     using Q'2 Conc' by blast
 qed
 
-(*
-  next, we need to decide how we want to represent the path constraints
-  probably "implies" is best.
-*)
+lemma childpath_rev_update_suffix :
+  assumes "childpath_rev_update cp upd = Some cp'"
+  shows "childpath_rev_update (cp@suf) upd = Some (cp'@suf)"
+  using assms
+proof(induction cp arbitrary: suf)
+  case Nil
+  then show ?case by(cases upd; auto)
+next
+  case (Cons ch ct)
+  show ?case 
+  proof(cases upd)
+    case Parent
+    then show ?thesis
+      using Cons by(auto)
+  next
+    case (Desc x2)
+    then show ?thesis
+      using Cons by(auto)
+  qed
+qed
 
-(* should we constrain P? 
-   "there is a satisfying assignment for any path"?
-*)
+lemma childpath_rev_update_None :
+  assumes H: "childpath_rev_update cp upd = None"
+  shows "upd = Parent" "cp = []"
+proof(cases cp)
+  case Nil
+  {
+    show "upd = Parent" using Nil H by(cases upd; auto)
+  }
+next
+  case (Cons a list)
+  {
+    have "False" using Cons H by(cases upd; auto)
+    thus "upd = Parent" by auto
+  }
+next
+  show "cp = []" using H by(cases cp; cases upd; auto)
+qed
 
-(* another option is just to use liftings here.
-   the problem with that is that these liftings tend to modify
-   other things *)
+lemma childpath_rev_update_suffix_None :
+  assumes H: "childpath_rev_update cp upd = None"
+  shows "childpath_rev_update (cp@(sufh#suft)) upd = Some suft" using assms
+proof(cases cp)
+  case Nil
+  then show ?thesis using H
+    by(cases upd; auto)
+next
+  case (Cons a list)
+  then show ?thesis using H
+    by(cases upd; auto)
+qed
+
+lemma childpath_update_prefix :
+  assumes H: "childpath_update cp upd = Some cp'"
+  shows "childpath_update (pref@cp) upd = Some (pref@cp')"
+proof-
+
+  show "childpath_update (pref @ cp) upd = Some (pref @ cp')"
+    using H childpath_rev_update_suffix 
+  unfolding childpath_update_def
+  by(auto split:option.splits)
+qed
+
+lemma childpath_update_None :
+  assumes H: "childpath_update cp upd = None"
+  shows "upd = Parent" "cp = []"
+proof-
+  have H' : "childpath_rev_update (rev cp) upd = None"
+    using H
+    unfolding childpath_update_def
+    by(auto split:option.split_asm)
+
+  show "upd = Parent"
+    using childpath_rev_update_None[OF H'] by auto
+
+  show "cp = []"
+    using childpath_rev_update_None[OF H'] by auto
+qed
 
 
-(*
-lemma vtsm_ctx :
-  assumes H0 : "gs_sem f' = f"
-  assumes Hp : "gensyn_get prog1 p = Some prog2"
+lemma childpath_update_prefix_None :
+  assumes H: "childpath_update cp upd = None"
+  shows "childpath_update ((prefb@[preft])@cp) upd = Some prefb" 
+proof-
+  obtain sufh suft where Suf :
+    "rev((prefb@[preft])) = sufh#suft"
+    by(cases "rev(prefb@[preft])"; auto)
 
-ok, we do need to (?) distinguish a "halt because we ran out of program" state
-*)
+  have H' : "childpath_rev_update (rev cp) upd = None"
+    using H unfolding childpath_update_def
+    by(auto split:option.splits)
 
-definition path_shift ::
-  "('x, 'mstate) g_sem \<Rightarrow>
-   (childpath \<Rightarrow> childpath) \<Rightarrow>
-   ('mstate \<Rightarrow> bool) \<Rightarrow>
-   ('mstate \<Rightarrow> bool) \<Rightarrow>
-   bool" where
-"path_shift f cpt P P' =
-  (\<forall> st p . P st \<longrightarrow>
-            gs_getpath f st = Some p \<longrightarrow>
-            (\<exists> st'. P' st' \<and> gs_getpath f st' = Some (cpt p)))"
+  have Upd' : "childpath_rev_update ((rev cp)@(sufh#suft)) upd = Some suft"
+    using childpath_rev_update_suffix_None[OF H'] by auto
 
-lemma path_shiftE [elim] :
-  assumes H0 : "path_shift f cpt P P'"
-  assumes HP : "P st"
-  assumes Hpath : "gs_getpath f st = Some p"
-  obtains st' where
-    "P' st'" "gs_getpath f st' = Some (cpt p)"
-  using assms unfolding path_shift_def by auto
-          
-
-lemma vtsm_sub :
-  assumes Hp : "gensyn_get prog1 ppre = Some prog2"
-
-  assumes HPP' :
-    "\<And> st psuf . P st \<Longrightarrow> gs_getpath f' st = Some (ppre @ psuf) \<Longrightarrow> P' st"
-
-  assumes Exc : "|? f' ?| %% {? P' ?}
-                             prog2
-                             {? Q' ?}"
-  
-  shows "|? f' ?| %% {? (\<lambda> st . P st \<and> gs_getpath f' st = Some (ppre@p))?}
-                     prog1
-                     {? (\<lambda> st . Q st \<and> gs_getpath f' st = Some (ppre@p'))?}"
-proof
-  fix st1
-  assume Hin : "P st1 \<and> gs_getpath f' st1 = Some (ppre @ p)"
-  hence Hin1 : "P st1" and Hin2 : "gs_getpath f' st1 = Some (ppre @ p)"
+  have Rev : "(rev ((prefb@[preft]) @ cp)) = (rev cp @ rev (prefb@[preft]))"
     by auto
 
-  (* hmmmmmm.... *)
+  show "childpath_update ((prefb@[preft]) @ cp) upd = Some prefb" using Upd'
+    unfolding childpath_update_def Rev using Suf
+    by(auto)
+qed
 
-  have HP' : "P' st1" using HPP'[OF Hin1 Hin2] by auto
+lemma droplast'_snoc :
+  "droplast' (l @ [x]) = l"
+proof(induction l arbitrary: x)
+case Nil
+  then show ?case by auto
+next
+  case (Cons a l)
+  then show ?case by(cases l; auto)
+qed
 
-  obtain n1 st'1 where 
-    Ex2 : "gensyn_sem_small_exec_many f' prog2 n1 st'1 = (st', Ok)" and
-    Post2 :
+lemma droplast_snoc :
+  "droplast (l @ [x]) = Some l"
+proof(induction l arbitrary: x)
+case Nil
+  then show ?case by auto
+next
+  case (Cons a l)
+  then show ?case by(cases l; auto)
+qed
 
-  show "\<exists>n st'. gensyn_sem_small_exec_many f' prog1 n st1 = (st', Ok) \<and>
-                Q st' \<and> gs_getpath f' st' = Some (ppre @ p')"
-    using GVTE[OF Exc HP']
+lemma droplast_snoc_conv :
+  assumes H : "droplast l = Some l'"
+  shows "\<exists> x . l = (l' @ [x])" using assms
+proof(induction l arbitrary: l')
+case Nil
+  then show ?case by auto
+next
+  case (Cons a l)
+  then show ?case by(cases l; auto split:option.splits)
+qed
 
-lemma vtsm_sub :
+lemma cons_snoc :
+  "\<exists> xb xx . xh # xt = (xb @ [xx])"
+proof(induction xt arbitrary: xh)
+  case Nil
+  then show ?case by auto
+next
+  case (Cons a xt)
+
+  obtain xb1 xx where Xb : "a#xt = xb1 @ [xx]"
+    using Cons[of a] by auto
+
+  have Conc' : "xh # a # xt = xh#xb1 @ [xx]" using Xb
+    by(auto)
+
+  thus ?case by auto
+qed
+
+
+lemma gsxm_sub_steps :
   assumes Hp : "gensyn_get prog1 ppre = Some prog2"
-  assumes Exc : "|? f' ?| %% {? (\<lambda> st . P st \<and> gs_getpath f' st = Some p) ?}
-                             prog2
-                             {? (\<lambda> st . Q st \<and> gs_getpath f' st = Some p') ?}"
-  shows "|? f' ?| %% {? (\<lambda> st . P st \<and> gs_getpath f' st = Some (ppre@p))?}
-                     prog1
-                     {? (\<lambda> st . Q st \<and> gs_getpath f' st = Some (ppre@p'))?}"
+  assumes H: "gensyn_sem_small_exec_many f' cp1 prog2 n st1 = (st2, Ok cp2)"
+  shows "gensyn_sem_small_exec_many f' (ppre@cp1) prog1 n st1 = (st2, Ok (ppre@cp2))"
+  using assms
+proof(induction n arbitrary: cp1 st1 cp2 st2)
+  case 0
+  then show ?case
+    by(auto)
+next
+  case (Suc n)
+
+  then obtain xl xd where X : "gensyn_get prog2 cp1 = Some (G xl xd)"
+    by(cases "gensyn_get prog2 cp1"; auto)
+
+  have Comp : "gensyn_get prog1 (ppre @ cp1) = Some (G xl xd)"
+    using gensyn_get_comp[OF X Hp] by auto
+
+  obtain cp_next where Cnext :
+    "childpath_update cp1 (gs_getpath f' (gs_sem f' xl st1)) = Some cp_next"
+    using Suc.prems X 
+    by(cases "childpath_update cp1 (gs_getpath f' (gs_sem f' xl st1))"; auto simp add: Let_def)
+
+  have Next :
+    "gensyn_sem_small_exec_many f' cp_next prog2 n (gs_sem f' xl st1) = (st2, Ok cp2)"
+    using Suc.prems X Cnext
+    by(auto simp add: Let_def)
+
+  have Cp2_pre :
+    "childpath_update (ppre @ cp1) (gs_getpath f' (gs_sem f' xl st1)) = Some (ppre @ cp_next)"
+    using childpath_update_prefix[OF Cnext] by auto
+
+  show ?case using Suc.IH[OF Hp Next] Comp Cp2_pre
+    by(auto simp add: Let_def)
+qed
+
+lemma vtsm_sub_steps :
+  assumes Hp : "gensyn_get prog1 ppre = Some prog2"
+  assumes H : "|? f' ?| % {?cp1,P1?} prog2 {?Ok cp2,P2?}"
+  shows "|? f' ?| % {?(ppre@cp1),P1?} prog1 {?Ok (ppre@cp2),P2?}"
 proof
-  fix st1
-  assume Hin : "P st1 \<and> gs_getpath f' st1 = Some (ppre @ p)"
-  hence Hin1 : "P st1" and Hin2 : "gs_getpath f' st1 = Some (ppre @ p)"
-    by auto
+  fix st
+  assume Hin : "P1 st"
 
-  obtain st2 where "P st2 \<and> gs_getpath f' st2 = Some p"
+  obtain n st' where Exec : "gensyn_sem_small_exec_many f' cp1 prog2 n st = (st', Ok cp2)" and P2 : "P2 st'"
+    using GVTE[OF H Hin] by auto
 
-  obtain n st' where Exc' :"gensyn_sem_small_exec_many f' prog2 n st = (st', Ok)" and
-                     Q' : "Q st'" and
-                     Path' : "gs_getpath f' st' = Some p'"
-    using GVTE[OF Exc]
+  show "\<exists>n st'.
+             gensyn_sem_small_exec_many f' (ppre @ cp1) prog1 n st =
+             (st', Ok (ppre @ cp2)) \<and>
+             P2 st'"
+    using gsxm_sub_steps[OF Hp Exec] P2 by auto
+qed
 
+(* this lemma is "precise", but I'm not sure if it's as useful as the next one *)
+lemma gsxm_sub_halt_step :
+  assumes Hp : "gensyn_get prog1 ppre = Some prog2"
+  assumes Hdrop : "droplast ppre = Some ppre'"
+  assumes Hlast: "gensyn_sem_small_exec_many f' cp1 prog2 n st1 = (st2, Ok cp2)"
+  assumes Hhalt: "gensyn_sem_small_exec f' cp2 prog2 st2 = (st3, Halted)"
+  shows "gensyn_sem_small_exec_many f' (ppre@cp1) prog1 (Suc n) st1 = (st3, Ok ppre')"
+  using assms
+proof(induction n arbitrary: cp1 cp2 st1 st2 st3 ppre ppre' prog1 prog2)
+  case 0
 
-  show "\<exists>n st'. gensyn_sem_small_exec_many f' prog1 n st = (st', Ok) \<and>
-                Q st' \<and> gs_getpath f' st' = Some (ppre @ p')"
+  then obtain xl xd where X : "gensyn_get prog2 cp1 = Some (G xl xd)"
+    by(cases "gensyn_get prog2 cp1"; auto)
 
+  have Comp : "gensyn_get prog1 (ppre @ cp1) = Some (G xl xd)"
+    using gensyn_get_comp[OF X] 0 by auto
 
-      using 
-    Exc' : 
+  have X' : "gensyn_get prog1 (ppre @ cp1) = Some (G xl xd)"
+    using 0 Comp X
+    by(cases "gensyn_get prog1 (ppre @ cp1)"; auto)
 
-(*
-  assumes Exc1' : "|? f'1 ?| % {{(\<lambda> st . P st \<and> gs_getpath f'1 st = p)}} 
-                               prog1
-                               {{(\<lambda> st . gs_getpath f'1 st = None)}}"
-  assumes Exc2 : "|! f'2 !| % {{(\<lambda> st . P st \<and> gs_getpath f'2 st = Some [])}} 
-                              prog2
-                              {{Q}}"
-  assumes Halt1 : "|! f'1 !| % {{(\<lambda> st . P st \<and> gs_getpath f'1 st = p)}} 
-                              prog1
-                              {{(\<lambda> st . gs_getpath f'1 st = None)}}"
-  shows Exc1 : "|! f'1 !| % {{(\<lambda> st . P st \<and> gs_getpath f'1 st = p)}} 
-                              prog1
-                            {{Q}}"
-*)
+  have Sub_None: "childpath_update cp2 (gs_getpath f' (gs_sem f' xl st2)) = None"
+    using 0 X Comp X'
+    by(auto split:option.splits simp add: Let_def)
 
-  (*assumes Hp2 : "gensyn_get x1 p = Some x2"*)
+  obtain ppreh ppret where Ppre_cons : "ppre = ppreh#ppret"
+    using "0.prems" by(cases ppre; auto)
+
+  obtain ppreb pprex where Ppre :
+    "ppre = ppreb @ [pprex]" using Ppre_cons cons_snoc[of ppreh ppret] by auto
+
+  have Ppre' : "ppreb = ppre'"
+    using 0 droplast_snoc[of ppreb pprex] Ppre by auto
     
-(* then we need a non-halting version of this *)
+  have Upd : "childpath_update (ppre@cp2) (gs_getpath f' (gs_sem f' xl st2)) = Some ppreb" 
+    using childpath_update_prefix_None[OF Sub_None, of ppreb pprex] Ppre
+    by(auto)
 
-(* OK, so new plan.
-- start with seq
-- relate behavior of sequence to individual ones using Hoare rules
-*)
+  show ?case using 0 X Comp X' Upd Ppre'
+    by(auto split:option.splits simp add: Let_def)
+next
+  case (Suc n)
 
-(*
- * mstate \<Rightarrow> childpath? just childpath?
- * mstate * unit gensyn * childpath list ?
- *)
-(*
-definition gVTS0 ::
-  "('x, 'mstate, 'xr) x_sem \<Rightarrow> 
-   ('mstate \<Rightarrow> childpath) \<Rightarrow>
-   ('mstate \<Rightarrow> bool) \<Rightarrow> 
-   'x gensyn \<Rightarrow>
-   ('mstate \<Rightarrow> bool) \<Rightarrow> 
-   bool"
-  (" |! _ @ _ !| !% {!_!} _ {!_!}")
-  where
-"gVTS0 sem getpath P syn Q =
-  (\<forall> st1 st2 n .
-    P st1 \<longrightarrow>
-    gensyn_sem_exec (sem) syn (getpath st1) st1 n = Some st2 \<longrightarrow>
-    Q st2)
-  "
-*)
-(*
-lemma VTS_gVTS :
-  assumes H : "sem % {{P}} x {{Q}}"
-  shows ""
-*)
+  then obtain xl xd where X : "gensyn_get prog2 cp1 = Some (G xl xd)"
+    by(cases "gensyn_get prog2 cp1"; auto)
 
-(* OK - my worry here is that when we merge states, we may not
-   be consistently getting the same thing out. *)
+  have Comp : "gensyn_get prog1 (ppre @ cp1) = Some (G xl xd)"
+    using gensyn_get_comp[OF X] Suc by auto
 
-(* one way to deal with this is to use the x_sem' structure (?)
-but it seems like maybe we are "throwing away" some information
-by using xsem operator, before we can use it to determine
-childpath... *)
+  have X' : "gensyn_get prog1 (ppre @ cp1) = Some (G xl xd)"
+    using Suc Comp X
+    by(cases "gensyn_get prog1 (ppre @ cp1)"; auto)
 
-(*
-multiple challenges here:
-1. lifting a single command
-2. lifting multiple commands
-- this could be interesting as, again, we are getting into the precise
-relationship between the small and big representation w/r/t child path
-*)
+  obtain ppreh ppret where Ppre_cons : "ppre = ppreh#ppret"
+    using "Suc.prems" by(cases ppre; auto)
+
+  obtain ppreb pprex where Ppre :
+    "ppre = ppreb @ [pprex]" using Ppre_cons cons_snoc[of ppreh ppret] by auto
+
+  have Ppre' : "ppreb = ppre'"
+    using Suc droplast_snoc[of ppreb pprex] Ppre by auto
+
+  show ?case
+  proof(cases "childpath_update cp1 (gs_getpath f' (gs_sem f' xl st1))")
+    case None
+    then show ?thesis 
+    proof(cases ppre)
+      case Nil
+      then show ?thesis
+        using Suc X Comp X' None
+        by(auto)
+    next
+      case (Cons ppreh ppret)
+      then show ?thesis
+        using Suc X Comp X' None
+        by(auto)
+    qed
+  next
+    case (Some cp1a)
+
+    show ?thesis
+    proof(cases "gensyn_get prog2 cp1a")
+      case None' : None
+      then show ?thesis 
+        using Some Suc.prems X Comp X' by(cases n; auto)
+    next
+      case Some' : (Some desc1a)
+
+      have Upd : "childpath_update (ppre@cp1) (gs_getpath f' (gs_sem f' xl st1)) = Some (ppre@cp1a)" 
+        using childpath_update_prefix[OF Some, of ppre] Ppre Ppre'
+        by(auto)
+
+      then show ?thesis using Some Suc  X Comp X'
+        by(auto split:option.splits simp add: Let_def)
+    qed
+  qed
+qed
+
+lemma vtsm_sub_halt_step :
+  assumes Hp : "gensyn_get prog1 ppre = Some prog2"
+  assumes Hdrop : "droplast ppre = Some ppre'"
+  assumes Hlast : "|? f' ?| % {?cp1, P1?} prog2 {?Ok cp2, P2?}"
+  assumes Hhalt: "\<And> st2 . P2 st2 \<Longrightarrow> 
+    \<exists> st3 . gensyn_sem_small_exec f' cp2 prog2 st2 = (st3, Halted) \<and> P3 st3"
+  shows "|? f' ?| % {? (ppre @ cp1), P1?} prog1 {? Ok ppre', P3?}"
+proof
+  fix st1
+  assume Hin : "P1 st1"
+
+  obtain n1 st2 where Exec1 : "gensyn_sem_small_exec_many f' cp1 prog2 n1 st1 =
+    (st2, Ok cp2)" and P2 : "P2 st2"
+    using GVTE[OF Hlast Hin] by auto
+
+  obtain st3 where Exec2 : "gensyn_sem_small_exec f' cp2 prog2 st2 = (st3, Halted)"
+    and P3 : "P3 st3"
+    using Hhalt[OF P2] by auto
+
+  have Conc' : "gensyn_sem_small_exec_many f' (ppre @ cp1) prog1 (Suc n1) st1 =
+                   (st3, Ok ppre') \<and> P3 st3"
+    using gsxm_sub_halt_step[OF Hp Hdrop Exec1 Exec2] P3
+    by auto
+
+  then show "\<exists>n st'.
+               gensyn_sem_small_exec_many f' (ppre @ cp1) prog1 n st1 =
+               (st', Ok ppre') \<and>
+               P3 st'"
+    by blast
+qed
+
+lemma gsxm_sub_halt :
+  assumes Hp : "gensyn_get prog1 ppre = Some prog2"
+  assumes Hdrop : "droplast ppre = Some ppre'"
+  assumes H: "gensyn_sem_small_exec_many f' cp1 prog2 n st1 = (st2, Halted)"
+  shows "(\<exists> n' . n' \<le> n \<and>
+            gensyn_sem_small_exec_many f' (ppre@cp1) prog1 n' st1 = (st2, Ok ppre'))"
+  using assms
+proof(induction n arbitrary: cp1 st1 st2 ppre ppre' prog1 prog2)
+  case 0
+  then show ?case
+    by(auto)
+next
+  case (Suc n)
+
+  then obtain xl xd where X : "gensyn_get prog2 cp1 = Some (G xl xd)"
+    by(cases "gensyn_get prog2 cp1"; auto)
+
+  have Comp : "gensyn_get prog1 (ppre @ cp1) = Some (G xl xd)"
+    using gensyn_get_comp[OF X] Suc by auto
+
+  have X' : "gensyn_get prog1 (ppre @ cp1) = Some (G xl xd)"
+    using Suc Comp X
+    by(cases "gensyn_get prog1 (ppre @ cp1)"; auto)
+
+  show ?case using Suc
+  proof(cases "childpath_update cp1 (gs_getpath f' (gs_sem f' xl st1))")
+    case None
+
+    show ?thesis
+    proof(cases ppre)
+      case Nil
+      then show ?thesis
+        using Suc X Comp X' None
+        by(auto)
+    next
+      case (Cons ppreh ppret)
+
+      obtain ppreb pprex where Ppre :
+        "ppre = ppreb @ [pprex]" using Cons cons_snoc[of ppreh ppret] by auto
+
+      have Ppre' : "ppreb = ppre'"
+        using Suc.prems(2) droplast_snoc[of ppreb pprex] Ppre by auto
+        
+      have Upd : "childpath_update (ppre@cp1) (gs_getpath f' (gs_sem f' xl st1)) = Some ppreb" 
+        using childpath_update_prefix_None[OF None, of ppreb pprex] Ppre
+        by(auto)
+
+      have CpNil : "cp1 = []" and Par : "(gs_getpath f' (gs_sem f' xl st1)) = Parent"
+        using childpath_update_None[OF None] by auto
+
+      (* in this case we halt immediately. *)
+      have Conc'1 : "gensyn_sem_small_exec_many f' (ppre @ cp1)
+        prog1 1 st1 =
+       (st2, Ok ppre')"
+        using Upd Cons None Comp X X' Ppre Suc.prems CpNil Par Ppre'
+        by(auto)
+
+      have Conc'2 : "1 \<le> Suc n" by auto
+
+      show ?thesis using Conc'1 Conc'2 by auto
+    qed
+  next
+    case(Some cp1a)
+    show ?thesis
+    proof(cases "gensyn_get prog2 cp1a")
+      case None' : None
+      then show ?thesis 
+        using Some Suc.prems X Comp X' by(cases n; auto)
+    next
+      case Some' : (Some desc1a)
+
+      have Exec : "gensyn_sem_small_exec_many f' cp1a prog2 n (gs_sem f' xl st1) = (st2, Halted)"
+        using Some Suc.prems  X Comp X' 
+        by(auto split:option.splits simp add: Let_def)
+
+      have Upd : "childpath_update cp1 (gs_getpath f' (gs_sem f' xl st1)) = Some cp1a"
+        using Some Suc.prems  X Comp X' Some'
+        by(auto)
+
+      show ?thesis using Some Suc.prems  X Comp X' Suc.IH[OF Suc.prems(1) Suc.prems(2) Exec] Some'
+          childpath_update_prefix[OF Upd,of ppre]
+        by(auto)
+    qed
+  qed
+qed
+
+lemma vtsm_sub_halt :
+  assumes Hp : "gensyn_get prog1 ppre = Some prog2"
+  assumes Hdrop : "droplast ppre = Some ppre'"
+  assumes H : "|? f' ?| % {?cp1, P1?} prog2 {?Halted, P2?}"
+  shows "|? f' ?| % {?(ppre @ cp1), P1?} prog1 {?Ok ppre', P2?}"
+proof
+  fix st
+  assume Hin : "P1 st"
+
+  obtain n st' where Exec : "gensyn_sem_small_exec_many f' cp1 prog2 n st = (st', Halted)"
+    and P2 : "P2 st'"
+    using GVTE[OF H Hin] by auto
+
+  obtain n' where Exec' :
+    "gensyn_sem_small_exec_many f' (ppre @ cp1) prog1 n' st = (st', Ok ppre')"
+    using gsxm_sub_halt[OF Hp Hdrop Exec] by auto
+
+  show "\<exists>n st'.
+             gensyn_sem_small_exec_many f' (ppre @ cp1) prog1 n st =
+             (st', Ok ppre') \<and>
+             P2 st'"
+    using Exec' P2 by blast
+qed
+
 
 (* necessary theorems (sketch):
 1. for a single instruction Hoare rule (assuming already lifted):
 in
 *)
 
-(*
-  can we phrase gVTS0 as VT?
-*)
 
 end
